Update `check_state` to consider only live data

compiler/backend/semantics/dataSemScript.sml
@@ -126,39 +126,70 @@ Definition size_of_heap_def:
 End
 
 
+Definition check2_res_def:
+  check2_res r (n, refs) =
+    if size refs <= size r then (n, refs) else (n, r)
+End
+
+Triviality check2_res_IMP:
+  !y. (n,r) = check2_res t y ==> size r <= size t
+Proof
+  fs [FORALL_PROD,check2_res_def] \\ rw []
+QED
+
+
 (* Checks if a value `dataSem$v` is within the limits set by the state:
 
    * The length of a Block fits in the header (< length_limit)
 
  *)
-val check_v_def = tDefine"check_v"`
-  check_v ^s (Block _ _ vl) =
-    (if LENGTH vl < s.limits.length_limit ** 32
-     then EVERY (check_v s) vl
-     else F)
-∧ check_v s _ = T`
-(WF_REL_TAC `measure (λ(ts,v). v_size v)`
- \\ `∀l. v1_size l = SUM (MAP (λx. v_size x + 1) l)`
-    by (Induct >> rw [definition"v_size_def"])
- \\ rw []
- \\ ho_match_mp_tac LESS_EQ_LESS_TRANS
- \\ Q.EXISTS_TAC `SUM (MAP (λx. v_size x + 1) vl)`
- \\ rw []
- \\ IMP_RES_TAC SUM_MAP_MEM_bound
- \\ ho_match_mp_tac LESS_EQ_TRANS
- \\ Q.EXISTS_TAC `v_size a + 1`
- \\ rw [])
 
-(* Checks the limits for all the values in the heap *)
+Definition check_v_def:
+  (check_v [] lim refs = (T, refs)) /\
+  (check_v (x::y::ys) lim refs  =
+    let (c1,refs1) = check2_res refs (check_v [x] lim refs) in
+    let (c2,refs2) = check_v (y::ys) lim refs1 in (c1 ∧ c2,refs2)) /\
+  (check_v [Word64 _]  lim refs = (T, refs)) /\
+  (check_v [Number _]  lim refs = (T, refs)) /\
+  (check_v [CodePtr _] lim refs = (T, refs)) /\
+  (check_v [RefPtr r]  lim refs =
+     case lookup r refs of
+     | NONE => (T, refs)
+     | SOME (ByteArray _ bs) => (T, delete r refs)
+     | SOME (ValueArray vs) =>  check_v vs lim (delete r refs)) /\
+  (check_v [Block ts tag vs] lim refs =
+     if LENGTH vs < lim ** 32 then
+       check_v vs lim refs
+     else (F,refs))
+Termination
+  WF_REL_TAC `(inv_image (measure I LEX measure v1_size)
+                          (\(vs,lin,refs). (sptree$size refs,vs)))`
+  \\ rpt strip_tac \\ fs [sptreeTheory.size_delete]
+  \\ imp_res_tac miscTheory.lookup_zero \\ fs []
+  \\ rw [] \\ fs []
+  \\ imp_res_tac check2_res_IMP \\ fs []
+End
+
+Triviality check2_res_check_v:
+  check2_res refs (check_v vs lim refs) = check_v vs lim refs
+Proof
+  qsuff_tac
+    `!vs lim refs. size (( \ (n,refs). refs) (check_v vs lim refs)) <= size refs`
+  THEN1 (rw [] \\ pop_assum (assume_tac o SPEC_ALL) \\ pairarg_tac \\ fs [check2_res_def])
+  \\ ho_match_mp_tac check_v_ind \\ fs [check_v_def] \\ rw []
+  \\ rpt (pairarg_tac \\ fs []) \\ rveq \\ fs[]
+  \\ fs [check2_res_def,bool_case_eq,option_case_eq,pair_case_eq,CaseEq"ref"]
+  \\ rveq \\ fs [] \\ rpt (pairarg_tac \\ fs []) \\ rveq \\ fs[] \\ fs [size_delete]
+QED
+
+Theorem size_of_def = REWRITE_RULE [check_res_size_of] size_of_def
+Theorem size_of_ind = REWRITE_RULE [check_res_size_of] size_of_ind
+
+(* Checks the limits for all the live values in the heap *)
 val check_state_def = Define`
   check_state ^s =
-  let locals_vs     = toList s.locals;
-      extract_stack = (λst. toList case st of Env vs => vs | Exc vs _ => vs);
-      extract_ref   = (λr. case r of ValueArray l =>  l | _ => []);
-      stack_vs      = FLAT (MAP extract_stack s.stack);
-      refs_vs       = FLAT (MAP extract_ref (toList s.refs));
-      all_vs        = locals_vs ++ stack_vs ++ refs_vs;
-  in EVERY (check_v s) all_vs
+    let (c,_) = check_v (stack_to_vs s) s.limits.length_limit s.refs
+    in c
 `
 
 Overload add_space_safe =
